finished the movies optimization.

theories/Demo.v
@@ -3,15 +3,119 @@ Require Import Coq.Strings.String.
 Require Import SemanticQuery.Types.
 Require Import SemanticQuery.Expr.
 Require Import SemanticQuery.Tables.
+Require Import SemanticQuery.RecordTableaux.
+Require Import SemanticQuery.Entailer.
+Require Import SemanticQuery.Chase.
+Require Import SemanticQuery.Minimize.
 Require Import SemanticQuery.Parsing.
 
 Set Implicit Arguments.
 Set Strict Implicit.
 
+Definition Row (r : row_type) : tuple typeD r -> row r := fun x => x.
+
+Module Movies.
+  Local Open Scope string_scope.
+
+  Definition tt_movies : row_type :=
+    (* title    : *) String ::
+    (* director : *) String ::
+    (* actor    : *) String :: nil.
+
+  Definition tbl_movies : table tt_movies :=
+    (Row tt_movies ("Star Trek: Into Darkness", ("JJ Abrams", ("Benedict Cumberbatch", tt)))) ::
+    (Row tt_movies ("Star Trek: Into Darkness", ("JJ Abrams", ("Chris Pine", tt)))) ::
+    (Row tt_movies ("Stardust", ("Matthew Vaughn", ("Claire Danes", tt)))) ::
+    (Row tt_movies ("Stardust", ("Matthew Vaughn", ("Robert Di Niro", tt)))) ::
+    (Row tt_movies ("Stardust", ("Matthew Vaughn", ("Charlie Cox", tt)))) :: nil.
+
+  Definition scheme := List.map Tuple (tt_movies :: nil).
+
+  Definition movies_db : DB scheme.
+    eapply Hcons.
+    eapply tbl_movies.
+    eapply Hnil.
+  Defined.
+
+  Notation "#0" := (@MZ _ _ _).
+  Notation "#1" := (@MN _ _ _ _ #0).
+  Notation "#2" := (@MN _ _ _ _ #1).
+
+  (** TODO: I need notation for this **)
+  Definition title_implies_director : embedded_dependency scheme :=
+    @Build_embedded_dependency scheme
+                               (Tuple tt_movies :: Tuple tt_movies :: nil)
+                               (Hcons #0 (Hcons #0 Hnil))
+                               (Expr.Eq (Expr.Proj (Expr.Var #0) #0) (Expr.Proj (Expr.Var #1) #0) :: nil)
+                               nil
+                               Hnil
+                               (Expr.Eq (Expr.Proj (Expr.Var #0) #1) (Expr.Proj (Expr.Var #1) #1) :: nil).
+(*
+  {| front_types := Tuple tt_movies :: Tuple tt_movies :: nil
+   ; front_binds := Hcons MZ (Hcons MZ Hnil)
+   ; front_filter := nil
+   ; back_types := nil
+   ; back_binds := Hnil
+   ; back_filter := nil
+   |}.
+*)
+
+  Theorem title_implies_director_sound
+  : embedded_dependencyD title_implies_director movies_db.
+  Proof.
+    red. simpl.
+  Admitted.
+
+  Example ex1 : query scheme (String :: String :: nil).
+  refine
+    (@Build_query scheme (String :: String :: nil)
+                      (QUERY scheme
+                       USING ("m1" <- 0 ;;
+                              ("m2" <- 0 ;;
+                              assert (Proj (Var "m1") 0) == (Proj (Var "m2") 0) ;;
+                              Ret)))
+                  (Hcons (Expr.Proj (Expr.Var #0) #1)
+                   (Hcons (Expr.Proj (Expr.Var #1) #2) Hnil))).
+  Defined.
+
+  Example universal_ex1 : query scheme (String :: String :: nil) :=
+    Eval vm_compute
+    in get_status (chase (@check_entails) 2 (title_implies_director :: nil) ex1).
+
+  Example minimized_ex1 : query scheme (String :: String :: nil) :=
+    Eval vm_compute
+    in minimize (@check_entails) universal_ex1.
+
+End Movies.
+
+(*
+Module Indexing.
+  Local Open Scope string_scope.
+
+  Definition tt_people : row_type :=
+    (* name : *) String ::
+    (* age  : *) Nat :: nil.
+
+  Definition tt_children : row_type :=
+    (* name : *) String ::
+    (* age  : *) Nat :: nil.
+
+  Definition scheme := List.map Tuple (tt_people :: tt_children :: nil).
+
+  Definition children_person : embedded_dependency scheme.
+  refine
+    (@Build_embedded_dependency scheme
+                               (Tuple tt_people :: nil)
+                               (Hcons #0 (Hcons #0 Hnil))
+                               (Expr.Eq (Expr.Proj (Expr.Var #0) #0) (Expr.Proj (Expr.Var #1) #0) :: nil)
+                               nil
+                               Hnil
+                               (Expr.Eq (Expr.Proj (Expr.Var #0) #1) (Expr.Proj (Expr.Var #1) #1) :: nil)).
+  
+
+
 Definition tt_names : row_type := Nat :: String :: nil.
 Definition tt_manager : row_type := Nat :: Nat :: nil.
-
-Definition Row (r : row_type) : tuple typeD r -> row r := fun x => x.
 
 Definition tbl_names : table tt_names :=
   (Row tt_names (0, ("Ryan"%string, tt))) ::
@@ -36,3 +140,4 @@ Goal True.
   unfold compile_q in t. simpl in t.
   exact I.
 Defined.
+*)
